theories/ml_toy_lang/iris/lang_instantiation.v
@@ -8,8 +8,8 @@ From melocoton.ml_toy_lang Require Export lang.
 
 
 (** Language *)
-Import ml_toy_lang.
-Lemma ml_toy_lang_mixin (p:ml_toy_lang.ml_program): ectxi_language.EctxiLanguageMixin of_val to_val fill_item head_step.
+Import ML_lang.
+Lemma ml_toy_lang_mixin (p:ML_lang.ml_program): ectxi_language.EctxiLanguageMixin of_val to_val fill_item head_step.
 Proof.
   split; apply _ || eauto using to_of_val, of_to_val, val_head_stuck,
     fill_item_val, fill_item_no_val_inj, head_ctx_step_val.
@@ -19,7 +19,7 @@ Canonical Structure ml_toy_ectx_lang p:= EctxLanguageOfEctxi (ml_toy_ectxi_lang 
 Canonical Structure ml_toy_lang p:= LanguageOfEctx (ml_toy_ectx_lang p).
 
 (* Prefer ml_toy_lang names over ectx_language names. *)
-Export ml_toy_lang.
+Export ML_lang.
 
 (** The following lemma is not provable using the axioms of [ectxi_language].
 The proof requires a case analysis over context items ([destruct i] on the
